src/SmtenIO.v
@@ -1,0 +1,80 @@
+
+Require Export Smten.
+Require Export SmtenProp.
+
+Module SmtenIO.
+Import Smten.Smten.
+Import SmtenProp.SmtenProp.
+
+Inductive valueio : tm -> Prop :=
+  | vio_return : forall t, valueio (treturnio t)
+  .
+
+Hint Constructors valueio.
+
+
+Reserved Notation "t1 '=IO=>' t2" (at level 40).
+
+Inductive stepio : tm -> tm -> Prop :=
+  | STIO_Pure : forall t t',
+      t ==> t' ->
+      t =IO=> t'
+  | STIO_BindReturn : forall t1 t2,
+      tbindio (treturnio t1) t2 =IO=> tapp t2 t1
+  | STIO_Bind : forall t1 t1' t2,
+      t1 =IO=> t1' ->
+      tbindio t1 t2 =IO=> tbindio t1' t2 
+
+where "t1 '=IO=>' t2" := (stepio t1 t2).
+
+Tactic Notation "stepio_cases" tactic(first) ident(c) :=
+  first;
+  [ Case_aux c "STIO_Pure" | Case_aux c "STIO_BindReturn"
+  | Case_aux c "STIO_Bind" ].
+
+Hint Constructors stepio.
+
+Notation multistepio := (multi stepio).
+Notation "t1 '=IO=>*' t2" := (multistepio t1 t2) (at level 40).
+
+
+Theorem progressio : forall t T,
+    empty |- t \in T ->
+    (exists T1 : ty, T = TIO T1) ->
+    valueio t \/ exists t', t =IO=> t'.
+
+Proof with eauto.
+  intros t T Ht HIOt.
+  remember (@empty ty) as Gamma.
+  has_type_cases (induction Ht) Case; subst Gamma...
+  Case "T_Var". inversion H.
+  Case "T_Abs". inversion HIOt. inversion H.
+  Case "T_App". 
+     (* progress says either tapp is a value or steps *)
+     destruct (progress (tapp t1 t2) T12)...
+     SCase "tapp is a value". inversion H.
+     SCase "tapp steps". right. destruct H as [t3]...
+  Case "T_Unit". inversion HIOt. inversion H.
+  Case "T_Pair". inversion HIOt. inversion H.
+  Case "T_Fst". 
+     destruct(progress (tfst t) T1)...
+     SCase "tfst is a value". inversion H.
+     SCase "tfst steps". right. destruct H as [t2]...
+  Case "T_Snd". 
+     destruct (progress (tsnd t) T2)...
+     SCase "tsnd is a value". inversion H.
+     SCase "tsnd steps". right. destruct H as [t2]...
+  Case "T_Inl". inversion HIOt. inversion H.
+  Case "T_Inr". inversion HIOt. inversion H.
+  Case "T_Case".
+     destruct (progress (tcase t1 t2 t3) T3)...
+     SCase "tcase is a value". inversion H.
+     SCase "tcase steps". right. destruct H as [t4]...
+  Case "T_BindIO".
+     right. destruct IHHt1...
+     SCase "t1 is a valueio". inversion H...
+     SCase "t1 is tbindio". destruct H as [t3]...
+Qed.
+
+End SmtenIO.
+
